finished example

coinduction-mwe-3.ec
@@ -1,24 +1,10 @@
-(* example proving a pRHL judgement relating structurally
-   dissimilar programs
-
-   the proof involves lots of symbolic evaluation
-
-   because the program executions settle into three mutually
-   recursive configurations, the proof involves mutual
-   induction *)
 
 prover quorum=2 ["Alt-Ergo" "Z3"].
 prover timeout=5.
 
 require import AllCore FSet.
 
-(* destinations: A, B and C - plus the environment *)
-
 type dest = [A | B | Env].
-
-(* an entity implements a procedure f taking in a destination and
-   integer, and returning a new integer plus the destination it should
-   be sent to *)
 
 module type ENT = {
   proc f(x : int) : dest * int
@@ -26,6 +12,321 @@ module type ENT = {
 
 
 section.
+
+
+declare module L <: ENT.
+declare module R <: ENT{-L}.
+
+module M = {
+  
+  proc a_loop(d : dest, x : int) : dest * int = {
+    while (d = A) { (d, x) <@ L.f(x); }
+    return (d, x);
+  }
+
+  proc b_loop(d : dest, x : int) : dest * int = {
+    while (d = B) { (d, x) <@ R.f(x); }
+    return (d, x);
+  }
+
+  proc run1(d : dest, x : int) : int = {
+    while (d = A \/ d = B) {
+      if (d = A) { (d, x) <@ L.f(x); }
+      else       { (d, x) <@ b_loop(d, x); }
+    }
+    return x;
+  }
+
+  proc run2(d : dest, x : int) : int = {
+    while (d = A \/ d = B) {
+      if (d = B) { (d, x) <@ R.f(x); } 
+      else       { (d, x) <@ a_loop(d, x); }
+    }
+    return x;
+  }
+
+  proc unroll1(d : dest, x : int) : int = {
+    (d, x) <@ b_loop(d, x);
+    x <@ run1(d, x);
+    return x;
+  }
+
+  proc unroll2(d : dest, x : int) : int = {
+    (d, x) <@ a_loop(d, x);
+    x <@ run2(d, x);
+    return x;
+  }
+}.
+
+op eq1 = equiv
+  [M.run1 ~ M.run2 :
+    ={d, x, glob L, glob R} ==>
+    ={res}].
+
+op eq2 = equiv
+  [M.run1 ~ M.unroll2 :
+    ={d, x, glob L, glob R} ==>
+    ={res}].
+
+op eq3 = equiv
+  [M.unroll1 ~ M.run2 :
+    ={d, x, glob L, glob R} ==>
+    ={res}].
+
+op IH = eq1 /\ eq2 /\ eq3.
+
+
+
+lemma ind1 : IH => eq1.
+proof.
+move => [_ [IH2 IH3]] @/eq1.
+proc.
+
+(* Env case *)
+case (d{1} = Env).
+rcondf{1} 1; auto.
+rcondf{2} 1; auto.
+
+
+(* A case *)
+case (d{1} = A).
+rcondt{1} 1 => //.
+rcondt{1} 1 => //.
+rcondt{2} 1 => //.
+rcondf{2} 1 => //.
+inline. sp.
+rcondt{2} 1 => //.
+seq 1 1 : (={glob L, glob R} /\ d{1} = d0{2} /\ x{1} = x0{2}).
+call (_ : true); auto.
+
+
+transitivity{1} {
+  x <@ M.run1(d,x);
+} (={d, x, glob L, glob R} ==> ={x})
+  (={glob L, glob R} /\ d{1} = d0{2} /\ x{1} = x0{2} ==> ={x}).
+progress. smt().
+smt().
+inline. sim.
+
+symmetry.
+transitivity{1} {
+  x <@ M.unroll2(d0,x0);
+} (={d0, x0, glob L, glob R} ==> ={x})
+  (={glob L, glob R} /\ d{2} = d0{1} /\ x{2} = x0{1} ==> ={x}).
+progress. smt().
+smt().
+inline. sim.
+symmetry.
+
+move : IH2 => @/eq2 IH2.
+call IH2 => //.
+
+
+(* B case *)
+conseq (_ : ={glob L, glob R, d, x} /\ d{1} = B ==> ={x}).
+smt().
+rcondt{1} 1 => //.
+rcondf{1} 1 => //.
+rcondt{2} 1 => //.
+rcondt{2} 1 => //.
+inline. sp.
+
+rcondt{1} 1 => //.
+seq 1 1 : (={glob L, glob R} /\ d0{1} = d{2} /\ x0{1} = x{2}).
+call (_ : true); auto.
+
+transitivity{1} {
+  x <@ M.unroll1(d0,x0);
+} (={d0, x0, glob L, glob R} ==> ={x})
+  (={glob L, glob R} /\ d0{1} = d{2} /\ x0{1} = x{2} ==> ={x}).
+progress. smt().
+smt().
+inline. sim.
+
+symmetry.
+transitivity{1} {
+  x <@ M.run2(d,x);
+} (={d, x, glob L, glob R} ==> ={x})
+  (={glob L, glob R} /\ d{1} = d0{2} /\ x{1} = x0{2} ==> ={x}).
+progress. smt().
+smt().
+inline. sim.
+symmetry.
+
+move : IH3 => @/eq3 IH3.
+call IH3 => //.
+
+qed.
+
+
+
+
+
+lemma ind2 : IH => eq2.
+proof.
+move => [_ [IH2 IH3]] @/eq2.
+proc.
+inline. wp. sp.
+
+(* Env case *)
+case (d{1} = Env).
+rcondf{1} 1; auto.
+rcondf{2} 1; auto.
+sp. rcondf{2} 1; auto.
+
+(* A case *)
+case (d{1} = A).
+rcondt{1} 1 => //.
+rcondt{1} 1 => //.
+rcondt{2} 1 => //.
+seq 1 1 : (={glob L, glob R} /\ d{1} = d0{2} /\ x{1} = x0{2}).
+call (_ : true); auto.
+
+transitivity{1} {
+  x <@ M.run1(d,x);
+} (={d, x, glob L, glob R} ==> ={x})
+  (={glob L, glob R} /\ d{1} = d0{2} /\ x{1} = x0{2} ==> x{1} = x1{2}).
+progress. smt().
+smt().
+inline. sim.
+
+symmetry.
+transitivity{1} {
+  x1 <@ M.unroll2(d0,x0);
+} (={d0, x0, glob L, glob R} ==> ={x1})
+  (={glob L, glob R} /\ d0{1} = d{2} /\ x0{1} = x{2} ==> x{2} = x1{1}).
+progress. smt().
+smt().
+inline. sim.
+symmetry.
+
+move : IH2 => @/eq2 IH2.
+call IH2 => //.
+
+(* B case *)
+conseq (_ : ={glob L, glob R, d, x} /\ d{1} = d0{2} /\ x{1} = x0{2} /\ d{1} = B ==> x{1} = x1{2}).
+progress. smt().
+rcondt{1} 1 => //.
+rcondf{1} 1 => //.
+rcondf{2} 1 => //.
+sp. elim* => ? ?.
+conseq (_ : ={glob L, glob R, d0, x0} /\ d0{1} = d1{2} /\ x0{1} = x1{2} /\ d0{1} = B 
+    ==> x{1} = x1{2}) => //.
+
+transitivity{1} {
+  x <@ M.unroll1(d0,x0);
+} (={glob L, glob R, d0, x0} ==> ={x})
+  (={glob L, glob R, d0, x0} /\ d0{1} = d1{2} /\ x0{1} = x1{2} /\ d0{1} = B ==> x{1} = x1{2}).
+progress. smt().
+smt().
+inline. sim.
+
+symmetry.
+transitivity{1} {
+  x1 <@ M.run2(d1,x1);
+} (={glob L, glob R, d1, x1} ==> ={x1})
+  (={glob L, glob R, d0, x0} /\ d0{2} = d1{1} /\ x0{2} = x1{1} ==> x{2} = x1{1}).
+progress. smt().
+smt().
+inline. sim.
+symmetry.
+
+move : IH3 => @/eq3 IH3.
+call IH3 => //.
+
+qed.
+
+
+lemma ind3 : IH => eq3.
+proof.
+move => [_ [IH2 IH3]] @/eq3.
+proc.
+inline. wp. sp.
+
+(* Env case *)
+case (d{1} = Env).
+rcondf{1} 1; auto.
+rcondf{2} 1; auto.
+sp. rcondf{1} 1; auto.
+
+(* B case *)
+case (d{1} = B).
+rcondt{1} 1 => //.
+rcondt{2} 1 => //.
+rcondt{2} 1 => //.
+seq 1 1 : (={glob L, glob R} /\ d0{1} = d{2} /\ x0{1} = x{2}).
+call (_ : true); auto.
+
+transitivity{1} {
+  x1 <@ M.unroll1(d0,x0);
+} (={d0, x0, glob L, glob R} ==> ={x1})
+  (={glob L, glob R} /\ d0{1} = d{2} /\ x0{1} = x{2} ==> x1{1} = x{2}).
+progress. smt().
+smt().
+inline. sim.
+
+symmetry.
+transitivity{1} {
+  x <@ M.run2(d,x);
+} (={glob L, glob R, d, x} ==> ={x})
+  (={glob L, glob R} /\ d0{2} = d{1} /\ x0{2} = x{1} ==> x1{2} = x{1}).
+progress. smt().
+smt().
+inline. sim.
+symmetry.
+
+move : IH3 => @/eq3 IH3.
+call IH3 => //.
+
+(* A case *)
+conseq (_ : ={glob L, glob R, d, x} /\ d0{1} = d{2} /\ x0{1} = x{2} /\ d{1} = A ==> x1{1} = x{2}).
+progress. smt().
+rcondt{2} 1 => //.
+rcondf{2} 1 => //.
+rcondf{1} 1 => //.
+sp. elim* => ? ?.
+conseq (_ : ={glob L, glob R, d0, x0} /\ d1{1} = d0{2} /\ x1{1} = x0{2} /\ d0{1} = A 
+    ==> x1{1} = x{2}) => //.
+
+transitivity{1} {
+  x1 <@ M.run1(d1,x1);
+} (={glob L, glob R, d1, x1} ==> ={x1})
+  (={glob L, glob R, d0, x0} /\ d1{1} = d0{2} /\ x1{1} = x0{2} /\ d0{1} = A ==> x1{1} = x{2}).
+progress. smt().
+smt().
+inline. sim.
+
+symmetry.
+transitivity{1} {
+  x <@ M.unroll2(d0,x0);
+} (={glob L, glob R, d0, x0} ==> ={x})
+  (={glob L, glob R, d0, x0} /\ d1{2} = d0{1} /\ x1{2} = x0{1} ==> x1{2} = x{1}).
+progress. smt().
+smt().
+inline. sim.
+symmetry.
+
+move : IH2 => @/eq2 IH2.
+call IH2 => //.
+
+qed.
+
+
+axiom lob H : (H => H) => H.
+
+
+lemma overall : eq1.
+proof.
+have H : (eq1 /\ eq2 /\ eq3 => eq1). auto.
+apply H. clear H.
+apply lob => IH.
+split; last split.
+by apply ind1.
+by apply ind2.
+by apply ind3.
+qed.
+
+
 
 abstract theory M.
 
@@ -77,6 +378,8 @@ clone M as N.
 declare module L <: ENT{-N.M1, -N.M2}.
 declare module R <: ENT{-N.M1, -N.M2, -L}.
 
+lemma ind :
+    eq1 /\ eq2 /\ eq3 => eq1 /\ eq2 /\ eq3.
 
 lemma ind :
   equiv
